thys/Untyped_Lambda_Calculus/LC_Beta.thy
@@ -1,7 +1,7 @@
 (* Here we instantiate the general enhanced rule induction to beta reduction
 for the (untyped) lambda-calculus *)
 theory LC_Beta
-imports LC "Binders.Generic_Barendregt_Enhanced_Rule_Induction" "Prelim.Curry_LFP" "Prelim.More_Stream" LC_Head_Reduction
+  imports LC "Binders.Generic_Barendregt_Enhanced_Rule_Induction" "Prelim.Curry_LFP" "Prelim.More_Stream" LC_Head_Reduction
 begin
 
 (* INSTANTIATING THE ABSTRACT SETTING: *)
@@ -20,13 +20,8 @@ inductive step :: "trm \<Rightarrow> trm \<Rightarrow> bool" where
 | Xi: "step e e' \<Longrightarrow> step (Lam x e) (Lam x e')"
 
 binder_inductive step
-  subgoal for \<sigma> R B t  \<comment> \<open>equivariance\<close>
-    by (elim disj_forward case_prodE)
-      (auto simp: isPerm_def term.rrename_comps rrename_tvsubst_comp
-         | ((rule exI[of _ "\<sigma> _"] exI)+, (rule conjI)?, rule refl)
-         | ((rule exI[of _ "\<sigma> _"])+; auto))+
   subgoal premises prems for R B t1 t2  \<comment> \<open>refreshability\<close>
-    by (tactic \<open>refreshability_tac false
+    by (tactic \<open>refreshability_tac true
       [@{term "FFVars :: trm \<Rightarrow> var set"}, @{term "FFVars :: trm \<Rightarrow> var set"}]
       [@{term "rrename :: (var \<Rightarrow> var) \<Rightarrow> trm \<Rightarrow> trm"}, @{term "(\<lambda>f x. f x) :: (var \<Rightarrow> var) \<Rightarrow> var \<Rightarrow> var"}]
       [SOME [SOME 1, SOME 0, NONE], NONE, NONE, SOME [SOME 0, SOME 0, SOME 1]]
